



TARUN KAUSHIK

MATHEMATICS

FOR

UPSC CSE MAINS

ODE PART 2



TARUN KAUSHIK

① "Ordinary Differential Equation"

Degree and Order :-

Eg. $\left(\frac{d^2y}{dx^2}\right)^3 + \left(\frac{dy}{dx}\right)^5 + y = 5x$

Here Order = 2 ; Degree = 3

Solutions of Differential equations :-

① By variable - separable

② By Homogeneous equation i.e. $y = vx$

③ Linear equation

i.e. $\frac{dy}{dx} + Py = Qx$

I.F. = $e^{\int P dx}$

$\Rightarrow y \cdot (I.F.) = \int Q \cdot (I.F.) dx$

official :-

① Exact Differential Eqⁿ :-

$Mdx + Ndy = 0$

But $Mx + Ny \neq 0$

and $\frac{\partial M}{\partial y} = \frac{\partial N}{\partial x}$

Solⁿ

$\int M dx + \int N dy = 0$

↑ 'exclude terms containing x'

② I.F (Integrating factor) found by inspection :-

(i) $y dx + x dy = d(xy)$

(ii) $\frac{y dx - x dy}{y^2} = d\left(\frac{x}{y}\right)$

②

iii) $d\left(\tan^{-1} \frac{y}{x}\right) = \frac{x dy - y dx}{x^2 + y^2}$

iv) $d\left(\log\left(\frac{y}{x}\right)\right) = \frac{x dy - y dx}{xy}$

v) $d(\log xy) = \frac{x dy + y dx}{xy}$

③ I.F. for a Homogeneous Equations :-

$Mdx + Ndy = 0$ But $Mx + Ny \neq 0$

then I.F. = $\frac{1}{Mx + Ny}$

④ I.F. for $f_1(xy) y dx + f_2(xy) x dy = 0$

I.F. = $\frac{1}{Mx - Ny}$

⑤ for $Mdx + Ndy = 0$

i) $\frac{\frac{\partial M}{\partial y} - \frac{\partial N}{\partial x}}{N} = f(x)$ then I.F. = $e^{\int f(x) dx}$

ii) $\frac{\frac{\partial N}{\partial x} - \frac{\partial M}{\partial y}}{M} = f(y)$ then I.F. = $e^{\int f(y) dy}$

Orthogonal trajectory :-

i) Cartesian

↓

Replace $\frac{dy}{dx}$ by $-\frac{dx}{dy}$

ii) Polar

$\frac{dr}{d\theta} = -r^2 \frac{d\theta}{dr}$

After doing differentiation w.r.t. 'x' or 'y'.



TARUN KAUSHIK

③

Linear Differential Equations :-

→ Dependent variable & its derivative \Rightarrow 1st degree

Operator $D = \frac{d}{dx}$

→ [Sol.ⁿ \Rightarrow Complete Sol.ⁿ = CF + PI]

$$\begin{array}{c} \uparrow \\ \boxed{A.E = 0} \end{array}$$

Working rules :-

① All roots Real :-

i.e. $(D-m_1)(D-m_2)y = 0$

$D = m_1, m_2$

$$CF = c_1 e^{m_1 x} + c_2 e^{m_2 x}$$

②

Two roots real & equal :-

i.e. $D = m, m$

$$CF = (c_1 + c_2 x) e^{mx}$$

③

If two roots of the A.E are imaginary,

$m_1 = \alpha + i\beta$ and $m_2 = \alpha - i\beta$

$$CF = e^{\alpha x} (c_1 \cos \beta x + c_2 \sin \beta x)$$

$$c_1 = c_1 + c_2 \quad \& \quad f(c_1 - c_2) = c_2$$

④

④ If two pairs of imaginary roots be equal,

$m_1 = m_2 = \alpha + i\beta$; $m_3 = m_4 = \alpha - i\beta$

$$CF = e^{\alpha x} [(c_1 x + c_2) \cos \beta x + (c_3 x + c_4) \sin \beta x]$$

$\frac{1}{f(D)}$ operator :

$$1) f(D)y = x \Rightarrow \boxed{y = \frac{1}{f(D)} x}$$

$$2) \frac{1}{D} x = \int x dx$$

$$3) \frac{1}{D-a} x = e^{ax} \int x e^{-ax} dx$$

Rules for finding the particular integral :-

$$P.I = \frac{1}{f(D)} x$$

$$1) x = e^{ax} \Rightarrow P.I = \frac{1}{f(D)} e^{ax} = \frac{e^{ax}}{f(a)} \quad \text{if } f(a) \neq 0$$

Now if $f(a) = 0$ then

$$\left(x \frac{e^{ax}}{f(a)} \right) \Leftarrow \frac{f'(D)}{f'(a)} \text{ then put } \frac{f'(D)}{f'(a)} \text{ if } f'(a) \neq 0$$

$$2) x = \sin(ax+b)$$

$$P.I = \frac{1}{f(D)} \sin(ax+b) \quad \text{put } (D^2 = -a^2)$$

$$3) x = x^m$$

$$P.I = \frac{1}{f(D)} x x^m \quad \text{Simplify.}$$

5

Que:- $\frac{d^2y}{dx^2} - 2 \frac{dy}{dx} + y = x e^x \sin x$

Sol.ⁿ

AE: $(D^2 - 2D + 1)y = 0$

$\Rightarrow (D-1)^2 y = 0 \Rightarrow D = 1, 1$

CF = $(x C_1 + C_2) e^x$

PI = $\frac{1}{(D-1)^2} x e^x \sin x$

= $e^x \frac{1}{((D+1)-1)^2} x \sin x$

= $e^x \left(\frac{1}{D^2} (x \sin x) \right)$

= $e^x \cdot \frac{1}{D} \int x \sin x dx$

= $e^x \cdot \frac{1}{D} [x(\cos x) - (1)(-\sin x)]$

= $-e^x \int x \cos x dx + \int -\sin x dx$

= $-e^x [x \sin x + \cos x + \cos x]$

= $-e^x (x \sin x + 2 \cos x)$

CS = $(C_1 x + C_2) e^x - e^x (x \sin x + 2 \cos x)$



TARUN KAUSHIK

6

(2015): 10 marks

$x \cos x \frac{dy}{dx} + y(x \sin x + \cos x) = 1$

Sol.ⁿ

$\frac{dy}{dx} + y \left(\tan x + \frac{1}{x} \right) = \frac{\sec x}{x}$

\rightarrow This is a linear equation of form

$\frac{dy}{dx} + Py = Q$

$\Rightarrow IF = e^{\int \tan x + \frac{1}{x} dx} = e^{\log \sec x + \log x} = e^{\log x \sec x} = x \sec x$

Sol.ⁿ $\Rightarrow y \times x \sec x = \int x \sec x \times \frac{\sec x}{x} dx$

$xy \sec x = \int \sec^2 x dx$

$xy \sec x = \tan x + C$

$xy = \sin x + C \cos x$ Ans.

Q (2015) Solve this differential equation :-
10 marks

$(2xy^4 e^y + 2xy^3 + y) dx + (x^2 y^4 e^y + x^2 y^2 - 3x) dy = 0$

Solution:-

$\frac{\partial M}{\partial y} = 2xy^4 e^y + 8xy^3 e^y + 6xy^2 + 1$

$\frac{\partial N}{\partial x} = 2xy^4 e^y + 2xy^2 - 3$

Now $\frac{\partial N}{\partial x} - \frac{\partial M}{\partial y} = \frac{2xy^4 e^y - 2xy^2 - 3 - 2xy^4 e^y - 8xy^3 e^y - 6xy^2 + 1}{y(2xy^3 e^y + 2xy^2 + 1)}$

⑦

$$= \frac{-8xy^3e^y - 8xy^2 - 4}{y(2xy^3e^y + 2xy^2 + 1)}$$

$$= \frac{-4(2xy^3e^y + 2xy^2 + 1)}{y(2xy^3e^y + 2xy^2 + 1)} = \frac{-4}{y}$$

Now I.F. = $e^{\int \frac{4}{y} dy} = e^{-4 \log y} = \left(\frac{1}{y^4}\right)$

Now multiply by $\left(\frac{1}{y^4}\right)$; we get

$$\Rightarrow \int \left(2x e^y + \frac{2x}{y} + \frac{1}{y^3}\right) dy + \int \left(x^2 e^y - \frac{x^2}{y^2} - \frac{3x}{y^4}\right) dy = 0$$

Neglect terms
containing x

$$\Rightarrow \boxed{x^2 e^y + \frac{x^2}{y} + \frac{x}{y^3} = C} \text{ Ans.}$$

Q(2015): 12 Marks:

Find the constant 'a' so that $(x+y)^a$ is the I.F. of $(4x^2 + 2xy + 6y)dx + (2x^2 + 9y + 3x)dy = 0$ and hence solve the differential equations.

Sol.ⁿ Since I.F. is given as $(x+y)^a$ so on multiplication with it; we get a exact differential equation.

$$\text{So } M = (x+y)^a (4x^2 + 2xy + 6y) \quad \&$$

$$N = (x+y)^a (2x^2 + 9y + 3x)$$

⑧

$$\frac{\partial M}{\partial y} = (x+y)^a (2x+6) + a(x+y)^{a-1} (4x^2 + 2xy + 6y)$$

$$\frac{\partial N}{\partial x} = (x+y)^a (4x+3) + a(x+y)^{a-1} (2x^2 + 9y + 3x)$$

$$\therefore \frac{\partial M}{\partial y} = \frac{\partial N}{\partial x} \quad (\text{for Exact diff. eq.})$$

$$\Rightarrow (x+y)^a [2x+6-4x-3] = a(x+y)^{a-1} (-2x^2 + 2xy + 3y + 3x)$$

$$\Rightarrow \cancel{(x+y)^a} (-3-2x) = a \frac{(x+y)^a}{(x+y)} \times \cancel{(x+y)} (3-2x)$$

$$\Rightarrow \boxed{a = 1}$$

$$= \int (x+y)(-4x^2 + 2xy + 6y) dx + \int (x+y)(2x^2 + 9y + 3x) dy$$

Exclude x terms

$$= \int (4x^3 + 2x^2y + 6xy + 4x^2y + 2xy^2 + 6y^2) dx + \int 9y^2 dy$$

$$= \left[x^4 + \frac{2x^3y}{3} + 3x^2y + \frac{4x^3y}{3} + \frac{x^2y^2}{2} + 6xy^2 + 3y^3 + C \right] \text{ Ans.}$$

Q(2014): 20 Marks: $x^3 \frac{d^3y}{dx^3} + 3x^2 \frac{d^2y}{dx^2} + x \frac{dy}{dx} + 8y = 65 \cos(\log x)$

Sol.ⁿ Put $x \frac{d}{dx} = D$ and $x = e^z \Rightarrow z = \log x$

$$x^3 \frac{d^3}{dx^3} = D(D-1)(D-2) = D^3 - 3D^2 + 2D$$

$$x^2 \frac{d^2}{dx^2} = D(D-1) = D^2 - D$$



TARUN KAUSHIK



TARUN KAUSHIK

Q

$$\Rightarrow (D^3 - 3D^2 + 4D + 3D^2 - 3D + 8) y = 65 \cos 2z$$

$$\Rightarrow (D^3 + 8)y = 65 \cos 2z$$

$$\therefore \text{A.E.} \Rightarrow D^3 + 8 = 0 \Rightarrow D^3 + 2^3 = 0$$

$$(D+2)(D^2 - 2D + 4) = 0$$

$$\Rightarrow D = -2 \text{ and } D = \frac{2 \pm \sqrt{-12}}{2}$$

$$\Rightarrow D = -2 \text{ \& } D = 1 \pm i\sqrt{3}$$

$$\therefore \text{C.F.} = C_1 e^{-2z} + (C_2 \cos \sqrt{3}z + C_3 \sin \sqrt{3}z) e^z$$

$$\text{and } \text{C.F.} = C_1 x^{-2} + x (C_2 \cos(\sqrt{3} \log x) + C_3 \sin(\sqrt{3} \log x))$$

$$\text{P.I.} = \frac{65 \cos 2z}{D^3 + 8} = \frac{65 \cos 2z}{D^2(D+8)} = \frac{65 \cos 2z}{-D+8}$$

$$= \frac{65 \cos 2z}{8-D} = \frac{65 (8+D)}{8^2 - D^2} = \frac{65 (8+D) \cos 2z}{8^2 - (-1)}$$

$$= \frac{65}{65} [8 \cos 2z - \sin 2z] = 8 \cos (2 \log x) - \sin (2 \log x)$$

$$\text{Complete Sol.} = [C_1 x^{-2} + x (C_2 \cos(\sqrt{3} \log x) + C_3 \sin(\sqrt{3} \log x)) + 8 \cos (2 \log x) - \sin (2 \log x)] \text{ Ans.}$$

Q(2013): 13 Marks: Orthogonal Trajectory

$$x^n = a \sin \theta \quad \dots \dots \dots (1)$$

$$\text{Sol.}^n \quad x^n x^{n-1} \frac{dx}{d\theta} = a^n \cos \theta \quad \dots \dots \dots (2)$$

10

dividing eq. (1) / eq. (2); we get

$$\frac{x^n}{x^{n-1} \cdot \left(\frac{dx}{d\theta}\right)} = \tan \theta \Rightarrow x = \tan \theta \cdot \frac{dx}{d\theta}$$

$$\rightarrow \text{replace } \frac{dx}{d\theta} \text{ by } -x^2 \frac{d\theta}{dx}$$

$$\Rightarrow x = -x^2 \tan \theta \frac{d\theta}{dx} \Rightarrow \frac{-dx}{x} = \int \tan \theta d\theta$$

$$\Rightarrow -\log x = \frac{\log \sec \theta}{n} + \log c$$

$$\Rightarrow -n \log x = \log \sec \theta + \log c^n$$

$$\Rightarrow \log x^{-n} = \log c^n \sec \theta$$

$$\Rightarrow x^{-n} = c^n \sec \theta$$

$$\Rightarrow x^n = c^{-n} \cos \theta \Rightarrow \boxed{x^n = b \cos \theta} \text{ Ans.}$$

Q(2013): 10 Marks:- $(5x^3 + 12x^2 + 6y^2) dx + 6xy dy = 0$

$$\text{Sol.}^n \quad M = 5x^3 + 12x^2 + 6y^2 \quad ; \quad N = 6xy$$

$$\frac{\partial M}{\partial y} = 12y \quad ; \quad \frac{\partial N}{\partial x} = 6y$$

$$\text{Now } \frac{\frac{\partial M}{\partial y} - \frac{\partial N}{\partial x}}{N} = \frac{12y - 6y}{6xy} = \frac{6y}{6xy} = \frac{1}{x}$$

$$\text{I.F.} = e^{\int \frac{1}{x} dx} = e^{\log x} = \frac{1}{x} \quad \dots \dots \dots (3)$$

11

$$= \int (5x^4 + 12x^3 + 6xy^2) dx + \int 6x^2y dy \quad \text{exclude } x \text{ term}$$

$$= \boxed{x^5 + 3x^4 + 3x^2y^2 + C} \quad \text{Ans}$$

Que:-(2013) Method of variation of Parameters
10 Marks

$$\frac{d^2y}{dx^2} + a^2y = \sec ax$$

Sol.ⁿ $(D^2 + a^2)y = \sec ax \leftarrow X$

Now A.E. $D^2 + a^2 = 0 \Rightarrow D = \pm ia$

so $CF = \boxed{C_1 \cos ax + C_2 \sin ax}$
 $\uparrow \quad \quad \uparrow$
 $y_1 \quad \quad y_2$

$$PI = -y_1 \int \frac{y_2 X}{W} dx + y_2 \int \frac{y_1 X}{W} dx$$

$$= -\cos ax \int \frac{\sin ax \cdot \sec ax}{a} dx + \sin ax \int \frac{\cos ax \cdot \sec ax}{a} dx$$

$$\therefore W = \begin{vmatrix} y_1 & y_2 \\ y_1' & y_2' \end{vmatrix} = \begin{vmatrix} \cos ax & \sin ax \\ -a \sin ax & a \cos ax \end{vmatrix} = a$$

$$= -\frac{\cos ax}{a} \int \tan ax dx + \frac{\sin ax}{a} \int dx$$

$$= \frac{\cos ax}{a^2} (\log \cos ax) + \frac{x \sin ax}{a}$$

Now CS = CF + PI Ans

12



TARUN KAUSHIK

Que (2013): 15 Marks

Find the general solution of the equation

$$x^2 \frac{d^2y}{dx^2} + x \frac{dy}{dx} + y = \log x \sin(\log x)$$

Sol.ⁿ

$$(\theta(\theta-1) + \theta + 1)y = Z \sin Z \quad \because e^Z = x$$

$$(\theta^2 - \theta + \theta + 1)y = Z \sin Z$$

$$(\theta^2 + 1)y = Z \sin Z$$

$$A.E. = D^2 + 1 = 0 \Rightarrow CF = C_1 \cos Z + C_2 \sin Z$$

$$PI = \frac{1}{D^2 + 1} Z \sin Z = \text{I.P. of } \frac{1}{D^2 + 1} Z e^{iZ}$$

$$= \text{I.P. of } e^{iZ} \frac{1}{(D+i)^2 + 1} Z = \text{I.P. of } \frac{e^{iZ}}{2iD(1+\frac{D}{2i})} Z$$

$$= \text{I.P. of } \frac{e^{iZ}}{2i} \frac{1}{D} \left(1 + \frac{D}{2i}\right)^{-1} Z = \text{I.P. of } \frac{e^{iZ}}{2i} \frac{1}{D} \left[1 - \frac{D}{2i}\right] Z$$

$$= \text{I.P. of } \frac{e^{iZ}}{2i} \frac{1}{D} \left(Z - \frac{1}{2i}\right) = \text{I.P. of } \frac{e^{iZ}}{2i} \int \left(Z - \frac{1}{2i}\right) dz$$

$$= \text{I.P. of } \frac{e^{iZ}}{2i} \left(\frac{Z^2}{2} + \frac{iZ}{2}\right) = \text{I.P. of } -\frac{e^{iZ}}{2} \left(\frac{Z^2}{2} + \frac{iZ}{2}\right)$$

$$= \text{I.P. of } -\frac{1}{2} (\cos Z + i \sin Z) \left(\frac{Z^2}{2} + \frac{iZ}{2}\right)$$

$$= -\frac{Z^2}{4} \cos Z + \frac{Z}{4} \sin Z = -\frac{1}{4} (\log x)^2 \cos(\log x) + \frac{1}{4} \log x \sin(\log x)$$

$$\boxed{CS = CF + PI} \quad \text{Ans}$$



TARUN KAUSHIK

Q(2012): 20 Marks $y''' - y'' = 12x^2 + 6x$

Sol.ⁿ $(D^3 - D^2)y = 12x^2 + 6x$

$$AE = D^3 - D^2 = 0 \Rightarrow D^2(D-1) = 0$$

$$D = 0, 0, 1$$

$$CF = (C_1x + C_2)e^{0x} + C_3e^x$$

$$PI = \frac{1}{D^2(D-1)} (12x^2 + 6x)$$

$$= \frac{-1}{D^2} \left[(1-D)^{-1} (12x^2 + 6x) \right]$$

$$= \frac{-1}{D^2} \left((1 + D + D^2 + \dots) (12x^2 + 6x) \right)$$

$$= \frac{-1}{D^2} \left[12x^2 + 6x + 24x + 6 + 24 \right]$$

$$= \frac{-1}{D^2} [12x^2 + 30x + 30]$$

$$= \frac{-1}{D} \int 12x^2 + 30x + 30 \, dx = \frac{-1}{D} [4x^3 + 15x^2 + 30x] \quad (14)$$

$$= -(x^4 + 5x^3 + 15x^2)$$

$$CS = CF + PI = C_1x + C_2 + C_3e^x - (x^4 + 5x^3 + 15x^2)$$

Ans:

Q (2012): 12 Marks Orthogonal Trajectory

Sol.ⁿ

$$x^2 + y^2 = ax$$

$$2x + 2y \frac{dy}{dx} = a$$

$$\Rightarrow 2x + 2y \frac{dy}{dx} = \frac{x^2 + y^2}{x}$$

Now Replace $\frac{dy}{dx}$ by $-\frac{dx}{dy}$

$$2x - 2y \frac{dx}{dy} = \frac{x^2 + y^2}{x} \Rightarrow 2x^2 - 2xy \frac{dx}{dy} = x^2 + y^2$$

$$\Rightarrow x^2 - y^2 = 2xy \frac{dx}{dy} \Rightarrow \frac{dy}{dx} = \frac{2xy}{x^2 - y^2}$$

Writing this in polar coordinates:

$$x = r \cos \theta ; y = r \sin \theta$$

$$\Rightarrow x^2 + y^2 = ax$$

$$\Rightarrow r^2 = ar \cos \theta \Rightarrow r = a \cos \theta$$

$$\Rightarrow \frac{dr}{d\theta} = -a \sin \theta \Rightarrow -r \frac{d\theta}{dr} = -r \tan \theta$$

$$\Rightarrow r \frac{d\theta}{dr} = \tan \theta \Rightarrow \int \cot \theta d\theta = \int \frac{dr}{r}$$

$$\Rightarrow \log \sin \theta = \log cr \Rightarrow cr = \sin \theta$$

$$\Rightarrow \boxed{r = b \sin \theta}$$

Now $r^2 = r b \sin \theta$

$$\Rightarrow \boxed{x^2 + y^2 = by} \text{ Ans.}$$

No Need.

Q (2012): 12 Marks

Solve

$$\frac{dy}{dx} = \frac{2xy e^{(x/y)^2}}{y^2 (1 + e^{(x/y)^2}) + 2x^2 e^{(x/y)^2}}$$

Sol.ⁿ

Put $x = vy \Rightarrow \frac{dx}{dy} = v + y \frac{dv}{dy}$

or $\boxed{v = x/y}$

$$\Rightarrow v + y \frac{dv}{dy} = \left(\frac{2ve^{v^2}}{1 + e^{v^2} + 2v^2 e^{v^2}} \right)^{-1}$$

$$\Rightarrow y \frac{dv}{dy} = \left(\frac{2ve^{v^2}}{1 + e^{v^2} + 2v^2 e^{v^2}} \right)^{-1} = \frac{1 + e^{v^2} + 2v^2 e^{v^2}}{2ve^{v^2}} - v$$

$$\Rightarrow y \frac{dv}{dy} = \frac{1 + e^{v^2} + 2v^2 e^{v^2} - 2v^2 e^{v^2}}{2ve^{v^2}}$$

$$\Rightarrow \int \frac{2ve^{v^2}}{1 + e^{v^2}} dv = \int \frac{dy}{y}$$

Put $1 + e^{v^2} = t$

$$e^{v^2} \times 2v dv = dt$$

$$\int \frac{dt}{t} = \int \frac{dy}{y} \Rightarrow \log t = \log cy$$

$$t = cy$$

$$\Rightarrow \boxed{1 + e^{(x/y)^2} = cy} \text{ Ans.}$$



TARUN KAUSHIK

$\frac{dy}{dx}$ is equal to
y is a function of x, such that the differential coefficient

$\cos(x+y) + \sin(x+y)$. Find out a relation between x and y, which is free from any derivative/differential.

Q(2013): $\frac{dy}{dx} = \cos(x+y) + \sin(x+y)$

Sol.ⁿ Put $x+y = z \Rightarrow 1 + \frac{dy}{dx} = \frac{dz}{dx}$

$$\Rightarrow \frac{dy}{dx} = \frac{dz}{dx} - 1 \quad \text{--- (1)}$$

$$\text{and } \frac{dy}{dx} = \cos z + \sin z \quad \text{--- (2)}$$

equating eq. (1) & eq. (2) : we get

$$\Rightarrow \frac{dz}{dx} - 1 = \cos z + \sin z$$

$$\Rightarrow \frac{dz}{dx} = 1 + \cos z + \sin z$$

$$\Rightarrow \frac{dz}{1 + \cos z + \sin z} = dx$$

$$\Rightarrow \frac{dz}{\frac{1 + \tan^2 \frac{z}{2}}{1 + \tan^2 \frac{z}{2}} + \frac{2 \tan \frac{z}{2}}{1 + \tan^2 \frac{z}{2}}} = dx$$

$$\Rightarrow \frac{\sec^2 \frac{z}{2} dz}{1 + \tan^2 \frac{z}{2} + 1 - \tan^2 \frac{z}{2} + 2 \tan \frac{z}{2}} = dx$$

$$\Rightarrow \int \frac{\sec^2 \frac{z}{2} dz}{2(1 + \tan \frac{z}{2})} = \int dx$$

$$\text{Put } \tan \frac{z}{2} = t \Rightarrow \sec^2 \frac{z}{2} dz = 2 dt$$

$$= \int \frac{dt}{1+t} = \int dx$$

$$\Rightarrow \log|1+t| = x + C$$

UPSC
2013
10 Marks

$$\Rightarrow \log|1 + \tan \frac{z}{2}| = x + C$$

$$\text{Put } z = x + y$$

$$\Rightarrow \boxed{\log|1 + \tan \frac{x+y}{2}| = x + C} \text{ Ans.}$$



TARUN KAUSHIK



TARUN KAUSHIK

Q (2012): 12 Marks

Solve

$$\frac{dy}{dx} = \frac{2xy e^{(x/y)^2}}{y^2(1 + e^{(x/y)^2}) + 2x^2 e^{(x/y)^2}}$$

Sol.ⁿ

$$\text{Put } x = vy \Rightarrow \frac{dx}{dy} = v + y \frac{dv}{dy}$$

or $\boxed{v = x/y}$

$$\Rightarrow v + y \frac{dv}{dy} = \left(\frac{2ve^{v^2}}{1 + e^{v^2} + 2v^2e^{v^2}} \right)^{-1}$$

$$\Rightarrow y \frac{dv}{dy} = \left(\frac{2ve^{v^2}}{1 + e^{v^2} + 2v^2e^{v^2}} \right)^{-1} = \frac{1 + e^{v^2} + 2v^2e^{v^2}}{2ve^{v^2}} - v$$

$$\Rightarrow y \frac{dv}{dy} = \frac{1 + e^{v^2} + \cancel{2v^2e^{v^2}} - \cancel{2v^2e^{v^2}}}{2ve^{v^2}}$$

$$\Rightarrow \int \frac{2ve^{v^2}}{1 + e^{v^2}} dv = \int \frac{dy}{y}$$

$$\text{Put } 1 + e^{v^2} = t$$

$$e^{v^2} \times 2v dv = dt$$

$$\int \frac{dt}{t} = \int \frac{dy}{y} \Rightarrow \log t = \log cy$$

$$t = cy$$

$$\Rightarrow \boxed{1 + e^{(x/y)^2} = cy}$$

Ans.



TARUN KAUSHIK

THANKS